cuvee/src/cuvee/backend/Prove.scala
@@ -3,77 +3,50 @@ package cuvee.backend
 import cuvee.pure._
 import cuvee.smtlib.DeclareFun
 
+/** This class
+  *
+  * @param solver
+  *   SMT solver to use to check expressions
+  */
 class Prove(solver: Solver) {
-  def prove(prop: Prop, expect: Boolean = true): Prop = prop match {
-    case atom: Atom => prove(atom, expect)
-    case neg: Neg   => prove(neg, expect)
-    case pos: Pos   => prove(pos, expect)
+  def prove(prop: Prop): Prop = prop match {
+    case atom: Atom => prove(atom)
+    case neg: Neg   => prove(neg)
+    case pos: Pos   => prove(pos)
   }
 
-  def prove(atom: Atom, expect: Boolean): Atom = atom match {
-    case Atom(phi) if expect && solver.isTrue(phi) =>
-      Atom(True)
-
-    case Atom(phi) if !expect && solver.isFalse(phi) =>
-      Atom(False)
-
-    case _ =>
-      atom
+  def prove(atom: Atom): Atom = atom match {
+    case Atom(phi) =>
+      if (solver.isTrue(phi))
+        Atom(True)
+      else
+        atom
   }
 
-  def prove(pos: Pos, expect: Boolean): Pos = pos match {
+  def prove(pos: Pos): Pos = pos match {
     case atom: Atom =>
-      prove(atom, expect)
+      prove(atom)
 
     case Conj(Nil, neg) =>
-      val neg_ = conj(neg, expect)
+      val neg_ = conj(neg)
+      Conj(Nil, neg_)
 
-      neg_ match {
-        case Nil =>
-          Atom.t
-        case neg_ if neg_ contains Atom.f =>
-          Atom.f
-        case _ =>
-          Conj(Nil, neg_)
-      }
-
-    case Conj(xs, neg) =>
-      val re = Expr.fresh(xs)
-      val re_ = re map (_.swap)
-
-      val xs_ = xs rename re
-      val neg_ = neg map (_ rename re)
-
-      val neg__ = conj(neg_, expect)
-
-      val res = neg__ match {
-        case Nil =>
-          Atom.t
-        case _ if neg__ contains Atom.f =>
-          Atom.f
-        case _ =>
-          Conj(xs, neg__ map (_ rename re_))
-      }
-
-      if (xs.nonEmpty && expect && solver.isTrue(res.toExpr)) {
-        Atom.t
-      } else {
-        res
-      }
+    case conj: Conj =>
+      prove(Atom(conj.toExpr))
   }
 
-  def prove(neg: Neg, expect: Boolean): Neg = neg match {
+  def prove(neg: Neg): Neg = neg match {
     case atom: Atom =>
-      prove(atom, expect)
+      prove(atom)
 
+    // forall xs. /\ {ant} ==> \/ {suc}
     case Disj(xs, neg, pos) =>
       solver.scoped {
         // A Disj contains variables quantified by a forall quantifier (disj.xs).
         // Below, we'll split those variables from their declaration in the quantifier.
         // Decide how to rename the quantified variables
         val re = Expr.fresh(xs)
-        val re_ = re map (_.swap)
-
+        //
         val xs_ = xs rename re
         val neg_ = neg map (_ rename re)
         val pos_ = pos map (_ rename re)
@@ -82,70 +55,57 @@ class Prove(solver: Solver) {
         for (x <- xs_)
           solver.declare(DeclareFun(x.sexpr, Nil, x.typ))
 
-        // Filter out redundant assumptions, always expect true
-        val neg__ = conj(neg_, expect)
-
-        // Add assumptions to the solver
-        for (phi <- neg__)
+        for (phi <- neg_)
           solver.assert(phi.toExpr)
 
-        // Filter out redundant conclusions
-        val pos__ = disj(pos_, expect)
-
-        val res = pos__ match {
-          case Nil =>
-            Atom(False)
-          case _ if pos__ contains Atom.t =>
-            Atom.t
-          case _ =>
-            // Undo the substitution
-            Disj(xs, neg__ map (_ rename re_), pos__ map (_ rename re_))
-        }
-
-        if (xs.nonEmpty && !expect && solver.isFalse(res.toExpr)) {
-          Atom.f
+        if (pos.isEmpty && solver.isUnsat) {
+          // Empty succedent: the only option to close the proof
+          // is when the assumptions are already inconsistent.
+          // However, do not do this eagerly, because *typically*
+          // they are not inconsistent if we have a proper goal.
+          Atom(True)
         } else {
-          res
+          // Otherwise: Attempt to prove one formula of the succedent,
+          // will succeed anyway if the assumptions are already inconsistent
+          val pos__ = disj(pos_)
+          Disj(xs_, neg_, pos__)
         }
       }
   }
 
-  def disj(suc: List[Pos], expect: Boolean): List[Pos] = suc match {
-    case Nil if expect && solver.isUnsat =>
-      List(Atom.t)
-
+  def disj(suc: List[Pos]): List[Pos] = suc match {
     case Nil =>
       Nil
 
     case first :: rest =>
-      prove(first, expect = false) match {
-        case Atom.f =>
-          disj(rest, expect)
+      prove(first) match {
+        case first_ @ Atom(False) =>
+          disj(rest)
 
         case first_ =>
           solver.scoped {
+            // justification: A \/ B  <==>  (A \/ (!A ==> B))
             solver.assert(!first_.toExpr)
-            first :: disj(rest, expect)
+            first_ :: disj(rest)
           }
       }
   }
 
-  def conj(ant: List[Neg], expect: Boolean): List[Neg] = ant match {
-    case Nil if !expect && solver.isUnsat =>
-      List(Atom.f)
-
+  def conj(ant: List[Neg]): List[Neg] = ant match {
     case Nil =>
       Nil
 
     case first :: rest =>
-      prove(first, expect = true) match {
-        case Atom.t =>
-          conj(rest, expect)
+      prove(first) match {
+        case first_ @ Atom(True) =>
+          conj(rest)
 
         case first_ =>
+          // TODO: check if we need to scope this
           solver.scoped {
+            // justification: A /\ B  <==>  (A /\ (A ==> B))
             solver.assert(first_.toExpr)
-            first :: conj(rest, expect)
+            first_ :: conj(rest)
           }
       }
   }
