cuvee/src/cuvee/backend/ProveSimple.scala
@@ -1,0 +1,44 @@
+package cuvee.backend
+
+import cuvee.pure._
+import cuvee.smtlib.DeclareFun
+
+class ProveSimple(solver: Solver) {
+  import Simplifier._
+
+  def prove(expr: Expr): Expr = expr match {
+    case And(phis) =>
+      simplifyAnd(phis map prove)
+
+    case Imp(phi, psi) =>
+      solver.scoped {
+        solver.assert(phi)
+        val psi_ = prove(psi)
+        simplifyImp(phi, psi_)
+      }
+
+    case Forall(xs, body) =>
+      solver.scoped {
+        val re = Expr.fresh(xs)
+        val re_ = re map (_.swap)
+
+        val xs_ = xs rename re
+        val body_ = body rename re
+
+        for (Var(name, typ) <- xs_) {
+          val cmd = DeclareFun(name, Nil, typ)
+          solver.declare(cmd)
+        }
+
+        val body__ = prove(body_)
+
+        Forall(xs, body__ rename re_)
+      }
+
+    case _ if solver.isTrue(expr) =>
+      True
+
+    case _ =>
+      expr
+  }
+}
