examples/case_studies/proc.bpl
@@ -39,4 +39,45 @@ procedure summary1() {
     assert b == a0 + b0;
 }
 
+function contains(x: int, a: [int]int, i: int, n: int): bool {
+    exists k: int :: i <= k && k < n && a[k] == x
+}
 
+procedure lsearch(x: int, a: [int]int, n: int)
+{
+    assume 0 <= n;
+
+    var r: bool := false;
+    var i: int  := 0;
+
+    while(i < n)
+        decreases n - i;
+        invariant 0 <= i && i <= n && !r;
+        summary   r <==> old(contains(x, a, i, n));
+    {
+        if(x == a[i]) {
+            r := true;
+            break;
+        }
+        
+        i := i + 1;
+    }
+
+    assert r <==> contains(x, a, 0, n);
+}
+
+procedure copy(a: [int]int, n: int) returns (b: [int]int)
+{
+    assume 0 <= n;
+    var i: int  := 0;
+
+    while(i < n)
+        decreases n - i;
+        invariant 0 <= i && i <= n;
+    {
+        b := b[i := a[i]];
+        i := i + 1;
+    }
+
+
+}
