examples/case_studies/prover.bpl
@@ -3,5 +3,6 @@ const B: bool;
 const C: bool;
 
 axiom A;
+lemma A && B ==> B;
 lemma B ==> !A;
 lemma C || (B ==> !A);
